Expose automatic lemma for node validity maintenance

ind/DoublyLinkedListIface.fst
@@ -392,8 +392,8 @@ let dll_remove_mid #t d n =
 let auto_dll_remains_valid_upon_staying_unchanged h0 h1 l d =
   admit () // TODO: Need to prove a bunch of things to make this happen
 
-// let auto_node_remains_valid_upon_staying_unchanged h0 h1 l n =
-//   admit () // TODO: Need to prove a bunch of things to make this happen
+let auto_node_remains_valid_upon_staying_unchanged h0 h1 l n =
+  admit () // TODO: Need to prove a bunch of things to make this happen
 
 /// Properties of nodes inside and outside lists
 ///
